proofs/fstar/extraction/Libcrux.Kem.Kyber.Arithmetic.fsti
@@ -1,0 +1,138 @@
+module Libcrux.Kem.Kyber.Arithmetic
+#set-options "--fuel 0 --ifuel 1 --z3rlimit 15"
+open Core
+open FStar.Mul
+
+unfold
+let t_FieldElement = i32
+
+unfold
+let t_FieldElementTimesMontgomeryR = i32
+
+unfold
+let t_MontgomeryFieldElement = i32
+
+let v_BARRETT_MULTIPLIER: i64 = 20159L
+
+let v_BARRETT_SHIFT: i64 = 26L
+
+let v_BARRETT_R: i64 = 1L <<! v_BARRETT_SHIFT
+
+let v_INVERSE_OF_MODULUS_MOD_R: u32 = 62209ul
+
+let v_MONTGOMERY_R_SQUARED_MOD_FIELD_MODULUS: i32 = 1353l
+
+let v_MONTGOMERY_SHIFT: u8 = 16uy
+
+let v_MONTGOMERY_R: i32 = 1l <<! v_MONTGOMERY_SHIFT
+
+val get_n_least_significant_bits (n: u8) (value: u32)
+    : Prims.Pure u32
+      (requires n =. 4uy || n =. 5uy || n =. 10uy || n =. 11uy || n =. v_MONTGOMERY_SHIFT)
+      (ensures
+        fun result ->
+          let result:u32 = result in
+          result <. (Core.Num.impl__u32__pow 2ul (Core.Convert.f_into n <: u32) <: u32))
+
+val barrett_reduce (value: i32)
+    : Prims.Pure i32
+      (requires
+        (Core.Convert.f_from value <: i64) >. (Core.Ops.Arith.Neg.neg v_BARRETT_R <: i64) &&
+        (Core.Convert.f_from value <: i64) <. v_BARRETT_R)
+      (ensures
+        fun result ->
+          let result:i32 = result in
+          result >. (Core.Ops.Arith.Neg.neg Libcrux.Kem.Kyber.Constants.v_FIELD_MODULUS <: i32) &&
+          result <. Libcrux.Kem.Kyber.Constants.v_FIELD_MODULUS)
+
+
+
+val montgomery_reduce (value: i32)
+    : Prims.Pure i32
+      (requires
+        value >=.
+        ((Core.Ops.Arith.Neg.neg Libcrux.Kem.Kyber.Constants.v_FIELD_MODULUS <: i32) *!
+          v_MONTGOMERY_R
+          <:
+          i32) &&
+        value <=. (Libcrux.Kem.Kyber.Constants.v_FIELD_MODULUS *! v_MONTGOMERY_R <: i32))
+      (ensures
+        fun result ->
+          let result:i32 = result in
+          result >=.
+          ((Core.Ops.Arith.Neg.neg (3l *! Libcrux.Kem.Kyber.Constants.v_FIELD_MODULUS <: i32) <: i32
+            ) /!
+            2l
+            <:
+            i32) &&
+          result <=. ((3l *! Libcrux.Kem.Kyber.Constants.v_FIELD_MODULUS <: i32) /! 2l <: i32))
+
+
+val montgomery_multiply_sfe_by_fer (fe fer: i32) : i32
+
+val to_standard_domain (mfe: i32) : i32
+
+val to_unsigned_representative (fe: i32)
+    : Prims.Pure u16
+      (requires
+        fe >=. (Core.Ops.Arith.Neg.neg Libcrux.Kem.Kyber.Constants.v_FIELD_MODULUS <: i32) &&
+        fe <. Libcrux.Kem.Kyber.Constants.v_FIELD_MODULUS)
+      (ensures
+        fun result ->
+          let result:u16 = result in
+          result >=. 0us &&
+          result <. (cast (Libcrux.Kem.Kyber.Constants.v_FIELD_MODULUS <: i32) <: u16))
+
+type t_PolynomialRingElement = { f_coefficients:t_Array i32 (sz 256) }
+
+let impl__PolynomialRingElement__ZERO: t_PolynomialRingElement =
+  { f_coefficients = Rust_primitives.Hax.repeat 0l (sz 256) } <: t_PolynomialRingElement
+
+val add_to_ring_element (v_K: usize) (lhs rhs: t_PolynomialRingElement)
+    : Prims.Pure t_PolynomialRingElement
+      (requires
+        v_K >. sz 1 /\
+        v_K <. sz 4 /\
+        (cast (v_K <: usize) <: i32) >. 1l /\
+        Hax_lib.v_forall (fun i ->
+              let i:usize = i in
+              Hax_lib.implies (i <. Libcrux.Kem.Kyber.Constants.v_COEFFICIENTS_IN_RING_ELEMENT
+                  <:
+                  bool)
+                (fun _ -> ((Core.Num.impl__i32__abs (lhs.f_coefficients.[ i ] <: i32) <: i32) <=.
+                    (((cast (v_K <: usize) <: i32) -! 1l <: i32) *!
+                      Libcrux.Kem.Kyber.Constants.v_FIELD_MODULUS
+                      <:
+                      i32)
+                    <:
+                    bool) &&
+                  ((Core.Num.impl__i32__abs (rhs.f_coefficients.[ i ] <: i32) <: i32) <=.
+                    Libcrux.Kem.Kyber.Constants.v_FIELD_MODULUS
+                    <:
+                    bool))
+              <:
+              bool))
+      (ensures fun _ -> True)
+(*      
+      (ensures
+        fun result ->
+          let result:t_PolynomialRingElement = result in
+          Hax_lib.v_forall (fun i ->
+                let i:usize = i in
+                Hax_lib.implies (i <.
+                    (Core.Slice.impl__len (Rust_primitives.unsize result.f_coefficients
+                          <:
+                          t_Slice i32)
+                      <:
+                      usize)
+                    <:
+                    bool)
+                  (fun _ -> (Core.Num.impl__i32__abs (result.f_coefficients.[ i ] <: i32) <: i32) <=.
+                    ((cast (v_K <: usize) <: i32) *! Libcrux.Kem.Kyber.Constants.v_FIELD_MODULUS
+                      <:
+                      i32)
+                    <:
+                    bool)
+                <:
+                bool))
+*)
